B_Unification/list_util.v
@@ -1,0 +1,360 @@
+Require Import List.
+Import ListNotations.
+Require Import Arith.
+Import Nat.
+Require Import Sorting.
+Require Import Permutation.
+
+Fixpoint lex {T : Type} (cmp : T -> T -> comparison) (l1 l2 : list T)
+              : comparison :=
+  match l1, l2 with
+  | [], [] => Eq
+  | [], _ => Lt
+  | _, [] => Gt
+  | h1 :: t1, h2 :: t2 =>
+      match cmp h1 h2 with
+      | Eq => lex cmp t1 t2
+      | c => c
+      end
+  end.
+
+(** 
+    There are some important but relatively straightforward properties of this function
+    that are useful to prove. First, reflexivity: 
+  *)
+
+Lemma lex_nat_refl : forall (l : list nat), lex compare l l = Eq.
+Proof.
+  intros.
+  induction l.
+  - simpl. reflexivity.
+  - simpl. rewrite compare_refl. apply IHl.
+Qed.
+
+(** 
+    Next, antisymmetry. This allows us to take a predicate or hypothesis about the 
+    comparison of two polynomials and reverse it. For example, a < b implies b > a.
+  *)
+
+Lemma lex_nat_antisym : forall (l1 l2 : list nat),
+  lex compare l1 l2 = CompOpp (lex compare l2 l1).
+Proof.
+  intros l1.
+  induction l1.
+  - intros. simpl. destruct l2; reflexivity.
+  - intros. simpl. destruct l2.
+    + simpl. reflexivity.
+    + simpl. destruct (a ?= n) eqn:H;
+      rewrite compare_antisym in H;
+      rewrite CompOpp_iff in H; simpl in H;
+      rewrite H; simpl.
+      * apply IHl1.
+      * reflexivity.
+      * reflexivity.
+Qed.
+
+Lemma lex_eq : forall n m,
+  lex compare n m = Eq <-> n = m.
+Proof.
+  intros n. induction n; induction m; intros.
+  - split; reflexivity.
+  - split; intros; inversion H.
+  - split; intros; inversion H.
+  - split; intros; simpl in H.
+    + destruct (a ?= a0) eqn:Hcomp; try inversion H. f_equal.
+      * apply compare_eq_iff in Hcomp; auto.
+      * apply IHn. auto.
+    + inversion H. simpl. rewrite compare_refl.
+      rewrite <- H2. apply IHn. reflexivity.
+Qed.
+
+Lemma lex_neq : forall n m,
+  lex compare n m = Lt \/ lex compare n m = Gt <-> n <> m.
+Proof.
+  intros n. induction n; induction m.
+  - simpl. split; intro. inversion H; inversion H0. contradiction.
+  - simpl. split; intro. intro. inversion H0. auto.
+  - simpl. split; intro. intro. inversion H0. auto.
+  - clear IHm. split; intros.
+    + destruct H; intro; apply lex_eq in H0; rewrite H in H0; inversion H0.
+    + destruct (a ?= a0) eqn:Hcomp.
+      * simpl. rewrite Hcomp. apply IHn. apply compare_eq_iff in Hcomp.
+        rewrite Hcomp in H. intro. apply H. rewrite H0. reflexivity.
+      * left. simpl. rewrite Hcomp. reflexivity.
+      * right. simpl. rewrite Hcomp. reflexivity.
+Qed.
+
+Lemma lex_neq' : forall n m,
+  (lex compare n m = Lt -> n <> m) /\
+  (lex compare n m = Gt -> n <> m).
+Proof.
+  intros n m. split.
+  - intros. apply lex_neq. auto.
+  - intros. apply lex_neq. auto.
+Qed.
+
+Lemma lex_rev_eq : forall n m,
+  lex compare n m = Eq <-> lex compare m n = Eq.
+Proof.
+  intros n m. split; intro; rewrite lex_nat_antisym in H; unfold CompOpp in H.
+  - destruct (lex compare m n) eqn:H0; inversion H. reflexivity.
+  - destruct (lex compare n m) eqn:H0; inversion H. reflexivity.
+Qed.
+
+Lemma lex_rev_lt_gt : forall n m,
+  lex compare n m = Lt <-> lex compare m n = Gt.
+Proof.
+  intros n m. split; intro; rewrite lex_nat_antisym in H; unfold CompOpp in H.
+  - destruct (lex compare m n) eqn:H0; inversion H. reflexivity.
+  - destruct (lex compare n m) eqn:H0; inversion H. reflexivity.
+Qed.
+
+(** 
+    Lastly is a property over lists. The comparison of two lists stays the same
+    if the same new element is added onto the front of each list. Similarly, if
+    the item at the front of two lists is equal, removing it from both does not
+    chance the lists' comparison. 
+  *)
+
+Lemma lex_nat_cons : forall (l1 l2 : list nat) n,
+  lex compare l1 l2 = lex compare (n::l1) (n::l2).
+Proof.
+  intros. simpl. rewrite compare_refl. reflexivity.
+Qed.
+
+Hint Resolve lex_nat_refl lex_nat_antisym lex_nat_cons.
+
+
+
+
+Lemma lt_Transitive :
+  Relations_1.Transitive lt.
+Proof.
+  unfold Relations_1.Transitive. intros. apply lt_trans with (m:=y); auto.
+Qed.
+
+Lemma NoDup_neq : forall {X:Type} (m : list X) a b,
+  NoDup (a :: b :: m) -> 
+  a <> b.
+Proof.
+  intros X m a b Hdup. apply NoDup_cons_iff in Hdup as [].
+  apply NoDup_cons_iff in H0 as []. intro. apply H. simpl. auto.
+Qed.
+
+Lemma HdRel_le_lt : forall a m,
+  HdRel (fun n m => is_true (leb n m)) a m /\ NoDup (a::m) -> HdRel lt a m.
+Proof.
+  intros a m []. remember (fun n m => is_true (leb n m)) as le.
+  destruct m.
+  - apply HdRel_nil.
+  - apply HdRel_cons. apply HdRel_inv in H.
+    apply (NoDup_neq _ a n) in H0; intuition. rewrite Heqle in H.
+    unfold is_true in H. apply leb_le in H. destruct (a ?= n) eqn:Hcomp.
+    + apply compare_eq_iff in Hcomp. contradiction.
+    + apply compare_lt_iff in Hcomp. apply Hcomp.
+    + apply compare_gt_iff in Hcomp. apply leb_correct_conv in Hcomp.
+      apply leb_correct in H. rewrite H in Hcomp. inversion Hcomp.
+Qed.
+
+
+
+
+
+Fixpoint nodup_cancel {A} Aeq_dec (l : list A) : list A :=
+  match l with
+  | [] => []
+  | x::xs => 
+    let count := (count_occ Aeq_dec xs x) in 
+    let xs' := (remove Aeq_dec x (nodup_cancel Aeq_dec xs)) in
+    if (even count) then x::xs' else xs'
+  end.
+
+Lemma In_remove : forall {A:Type} Aeq_dec a b (l:list A),
+  In a (remove Aeq_dec b l) -> In a l.
+Proof.
+  intros A Aeq_dec a b l H. induction l as [|c l IHl].
+  - contradiction.
+  - destruct (Aeq_dec b c) eqn:Heq; simpl in H; rewrite Heq in H.
+    + right. auto.
+    + destruct H; [rewrite H; intuition | right; auto].
+Qed.
+
+Lemma Forall_cons_iff : forall (A:Type) Rel a (l:list A),
+  Forall Rel (a::l) <-> Forall Rel l /\ Rel a.
+Proof.
+  intros A Rel a l. split.
+  - intro H. split.
+    + rewrite Forall_forall in H. apply Forall_forall. intros x Hin.
+      apply H. intuition.
+    + apply Forall_inv in H. auto.
+  - intros []. apply Forall_cons; auto.
+Qed.
+
+Lemma Forall_remove : forall (A:Type) Aeq_dec Rel a (l:list A),
+  Forall Rel l -> Forall Rel (remove Aeq_dec a l).
+Proof.
+  intros A Aeq_dec Rel a l H. induction l.
+  - simpl. auto.
+  - simpl. apply Forall_cons_iff in H. destruct (Aeq_dec a a0).
+    + apply IHl. apply H.
+    + apply Forall_cons_iff. split.
+      * apply IHl. apply H.
+      * apply H.
+Qed.
+
+Lemma StronglySorted_remove : forall {A:Type} Aeq_dec Rel a (l:list A),
+  StronglySorted Rel l -> StronglySorted Rel (remove Aeq_dec a l).
+Proof.
+  intros A Aeq_dec Rel a l H. induction l.
+  - simpl. auto.
+  - simpl. apply StronglySorted_inv in H. destruct (Aeq_dec a a0).
+    + apply IHl. apply H.
+    + apply SSorted_cons.
+      * apply IHl. apply H.
+      * apply Forall_remove. apply H.
+Qed.
+
+Lemma not_In_remove : forall (A:Type) Aeq_dec a (l : list A),
+  ~ In a l -> (remove Aeq_dec a l) = l.
+Proof.
+  intros A Aeq_dec a l H. induction l.
+  - simpl. reflexivity.
+  - simpl. destruct (Aeq_dec a a0).
+    + simpl. rewrite e in H. exfalso. apply H. intuition.
+    + rewrite IHl. reflexivity. intro Hin. apply H. intuition.
+Qed.
+
+Lemma remove_distr_app : forall (A:Type) Aeq_dec x (l l':list A),
+  remove Aeq_dec x (l ++ l') = remove Aeq_dec x l ++ remove Aeq_dec x l'.
+Proof.
+  intros A Aeq_dec x l l'. induction l; intros.
+  - simpl. auto.
+  - simpl. destruct (Aeq_dec x a).
+    + apply IHl.
+    + simpl. f_equal. apply IHl.
+Qed.
+
+Lemma nodup_cancel_in : forall (A:Type) Aeq_dec a (l:list A),
+  In a (nodup_cancel Aeq_dec l) -> In a l.
+Proof.
+  intros A Aeq_dec a l H. induction l as [|b l IHl].
+  - contradiction.
+  - simpl in H. destruct (Aeq_dec a b).
+    + rewrite e. intuition.
+    + right. apply IHl. destruct (even (count_occ Aeq_dec l b)).
+      * simpl in H. destruct H. rewrite H in n. contradiction.
+        apply In_remove in H. auto.
+      * apply In_remove in H. auto.
+Qed.
+
+Lemma NoDup_remove : forall (A:Type) Aeq_dec a (l:list A),
+  NoDup l -> NoDup (remove Aeq_dec a l).
+Proof.
+  intros A Aeq_dec a l H. induction l.
+  - simpl. auto.
+  - simpl. destruct (Aeq_dec a a0).
+    + apply IHl. apply NoDup_cons_iff in H. intuition.
+    + apply NoDup_cons.
+      * apply NoDup_cons_iff in H as []. intro. apply H.
+        apply (In_remove Aeq_dec a0 a l H1).
+      * apply IHl. apply NoDup_cons_iff in H; intuition.
+Qed.
+
+Lemma NoDup_forall_neq : forall (A:Type) a (l:list A),
+  Forall (fun b => a <> b) l ->
+  NoDup l ->
+  NoDup (a :: l).
+Proof.
+  intros A a l Hf Hn. apply NoDup_cons.
+  - intro. induction l.
+    + inversion H.
+    + apply Forall_cons_iff in Hf as []. apply IHl.
+      * apply H0.
+      * apply NoDup_cons_iff in Hn. apply Hn.
+      * simpl in H. destruct H; auto. rewrite H in H1. contradiction.
+  - auto.
+Qed.
+
+Lemma NoDup_nodup_cancel : forall (A:Type) Aeq_dec (l:list A),
+NoDup (nodup_cancel Aeq_dec l).
+Proof.
+  induction l as [|a l' Hrec]; simpl.
+  - constructor.
+  - destruct (even (count_occ Aeq_dec l' a)); simpl.
+    + apply NoDup_cons; [apply remove_In | apply NoDup_remove; auto].
+    + apply NoDup_remove; auto.
+Qed.
+
+Lemma no_nodup_NoDup : forall (A:Type) Aeq_dec (l:list A),
+  NoDup l ->
+  nodup Aeq_dec l = l.
+Proof.
+  intros A Aeq_dec l H. induction l.
+  - auto.
+  - simpl. apply NoDup_cons_iff in H as []. destruct (in_dec Aeq_dec a l).
+    contradiction. f_equal. auto.
+Qed.
+
+Lemma no_nodup_cancel_NoDup : forall (A:Type) Aeq_dec (l:list A),
+  NoDup l ->
+  nodup_cancel Aeq_dec l = l.
+Proof.
+  intros A Aeq_dec l H. induction l.
+  - auto.
+  - simpl. apply NoDup_cons_iff in H as []. assert (count_occ Aeq_dec l a = 0).
+    + apply count_occ_not_In. auto.
+    + rewrite H1. simpl. f_equal. rewrite not_In_remove. auto. intro.
+      apply nodup_cancel_in in H2. apply H. auto.
+Qed.
+
+Lemma Sorted_nodup : forall (A:Type) Aeq_dec Rel (l:list A),
+  Relations_1.Transitive Rel ->
+  Sorted Rel l ->
+  Sorted Rel (nodup Aeq_dec l).
+Proof.
+  intros A Aeq_dec Rel l Ht H. apply Sorted_StronglySorted in H; auto.
+  apply StronglySorted_Sorted. induction l.
+  - auto.
+  - simpl. apply StronglySorted_inv in H as []. destruct (in_dec Aeq_dec a l).
+    + apply IHl. apply H.
+    + apply SSorted_cons.
+      * apply IHl. apply H.
+      * rewrite Forall_forall in H0. apply Forall_forall. intros x Hin.
+        apply H0. apply nodup_In in Hin. auto.
+Qed.
+
+Lemma Sorted_nodup_cancel : forall (A:Type) Aeq_dec Rel (l:list A),
+  Relations_1.Transitive Rel ->
+  Sorted Rel l -> 
+  Sorted Rel (nodup_cancel Aeq_dec l).
+Proof.
+  intros A Aeq_dec Rel l Ht H. apply Sorted_StronglySorted in H; auto.
+  apply StronglySorted_Sorted. induction l.
+  - auto.
+  - simpl. apply StronglySorted_inv in H as []. destruct (even (count_occ Aeq_dec l a)).
+    + apply SSorted_cons.
+      * apply StronglySorted_remove. apply IHl. apply H.
+      * apply Forall_remove. apply Forall_forall. rewrite Forall_forall in H0.
+        intros x Hin. apply H0. apply nodup_cancel_in in Hin. auto.
+    + apply StronglySorted_remove. apply IHl. apply H.
+Qed.
+
+Lemma count_occ_Permutation : forall (A:Type) Aeq_dec a (l l':list A),
+  Permutation l l' ->
+  count_occ Aeq_dec l a = count_occ Aeq_dec l' a.
+Proof.
+  intros A Aeq_dec a l l' H. induction H.
+  - auto.
+  - simpl. destruct (Aeq_dec x a); auto.
+  - simpl. destruct (Aeq_dec y a); destruct (Aeq_dec x a); auto.
+  - rewrite <- IHPermutation2. rewrite IHPermutation1. auto.
+Qed.
+
+Lemma Permutation_not_In : forall (A:Type) a (l l':list A),
+  Permutation l l' ->
+  ~ In a l ->
+  ~ In a l'.
+Proof.
+  intros A a l l' H H0. intro. apply H0. apply Permutation_sym in H.
+  apply (Permutation_in a) in H; auto.
+Qed.
